Core model working

spi_host/spi_hostCoreScript.sml
@@ -1,5 +1,6 @@
 open HolKernel Parse boolLib bossLib;
 open spi_hostRegsTheory;
+open BasicProvers;
 
 val _ = new_theory("spi_hostCore");
 
@@ -143,7 +144,7 @@ Definition spi_host_core_command:
 End
 
 Datatype:
-  delay = <|
+  spi_delay = <|
     csnlead   : 4 word;
     csntrail  : 4 word;
     csnidle   : 4 word;
@@ -181,7 +182,7 @@ Definition spi_host_tick_def:
       sw_rst_i: bool = word_bit 0 (st.regs.control.sw_rst);
       en_i: bool = ((st.regs.control.spien = 1w) ∧ spi_host_core_no_error(st.regs.error_status));
 
-      fsm_en = (en_i ∧ st.clock_counter = 0w);
+      fsm_en: bool = (en_i ∧ st.clock_counter = 0w);
       
       empty_command_update: spi_host_command_update = <|len:= 0w; csaat:= 0w; speed:= 0w; direction:= 0w; |>;
 
@@ -195,8 +196,10 @@ Definition spi_host_tick_def:
 
       next_command: command = HD st.commands;
 
-      command_ready_idle_csb_active: bool = if command_valid_i then ¬(next_command.csid = st.csid_q)
-                                              else T;
+      (* command_ready_idle_csb_active: bool = if command_valid_i then ¬(next_command.csid = st.csid_q)
+                                              else T; *)
+			(* This is a little hacky to reduce the complexity of HOL output *)		      
+      command_ready_idle_csb_active: bool = ¬(next_command.csid = st.csid_q);
 
       command_ready_int: bool = if st.fsm_state = Idle ∨ st.fsm_state = WaitIdle then T
                                 else if st.fsm_state = IntClockHigh ∨ st.fsm_state = IdleCSBActive then command_ready_idle_csb_active
@@ -205,16 +208,16 @@ Definition spi_host_tick_def:
 
       commands'' = if new_command then TL commands' else commands';
 
-      config' = if new_command ∧ (st.regs.csid.csid = 1w) then spi_host_configopts_0_to_configopts(st.regs.configopts_0)
-                  else st.config; 
+      config': configopts = if new_command ∧ (st.regs.csid.csid = 1w) then spi_host_configopts_0_to_configopts(st.regs.configopts_0)
+                            else st.config; 
 	    (* Could be good to have this all config opts maybe? But we are only dealling with one csid *)
 
-      cmd_speed' = if new_command then next_command.speed else st.cmd_speed;
+      cmd_speed': 2 word = if new_command then next_command.speed else st.cmd_speed;
 
       start_bit: 3 word = if cmd_speed' = 0w then 7w else if cmd_speed' = 1w then 6w else 4w;
       shift_size: 3 word = if cmd_speed' = 0w then 1w else if cmd_speed' = 1w then 2w else 4w;
 
-      switch_required = ¬(config' = st.config);
+      switch_required: bool = ¬(config' = st.config);
 
       clock_counter': 16 word = if sw_rst_i then 0w
                                 else if ¬en_i then st.clock_counter
@@ -222,25 +225,25 @@ Definition spi_host_tick_def:
                                 else if new_command then st.config.clkdiv
                                 else if (st.clock_counter = 0w) then st.config.clkdiv
                                 else st.clock_counter - 1w;
-      delay = <| 
+      delay: spi_delay = <|
         csnlead   := st.config.csnlead;
         csntrail  := st.config.csntrail;
         csnidle   := st.config.csnidle;
       |>;
 
-      last_bit = (st.bit_counter = 0w);
-      last_byte = (st.byte_counter = 0w);
+      last_bit: bool = (st.bit_counter = 0w);
+      last_byte: bool = (st.byte_counter = 0w);
 
-      state_after_idle =    if new_command then
-                              if switch_required then ConfigSwitch
-                              else WaitLead
-                            else Idle;
+      state_after_idle =  if new_command then
+                            if switch_required then ConfigSwitch
+                            else WaitLead
+                          else Idle;
       state_after_idle_csb_active = if new_command then
                                       if switch_required then WaitTrail
                                       else IntClockLow
                                     else IdleCSBActive;
 
-      fsm_state' = case st.fsm_state of 
+      fsm_state': fsmState = case st.fsm_state of
           Idle                =>  state_after_idle
         | ConfigSwitch        =>  if st.counter > 1w then ConfigSwitch
                                   else WaitLead
@@ -257,47 +260,47 @@ Definition spi_host_tick_def:
         | WaitIdle            =>  if st.counter > 1w then WaitIdle
                                   else state_after_idle;
 
-      curr_delay = case fsm_state' of 
+      curr_delay: 4 word = case fsm_state' of
           WaitLead => delay.csnlead
         | WaitTrail => delay.csntrail
         | WaitIdle => delay.csnidle
         | ConfigSwitch => delay.csnidle
         | _ => 0w;
 
-      state_changing = ¬(fsm_state' = st.fsm_state);
-      counter' = if state_changing then curr_delay 
-                 else if st.counter > 0w then st.counter - 1w 
-                 else 0w; 
+      state_changing: bool = ¬(fsm_state' = st.fsm_state);
+      counter': 4 word = if state_changing then curr_delay 
+                          else if st.counter > 0w then st.counter - 1w 
+                          else 0w; 
 
-      cpha = word_bit 0 st.config.cpha;
+      cpha: bool = word_bit 0 st.config.cpha;
       
-      byte_starting_cpha0' = (¬(sw_rst_i) ∧ state_changing ∧ 
-                            ((fsm_state' = WaitLead) ∨ (fsm_state' = IntClockLow ∧ st.bit_counter = 0w)));
+      byte_starting_cpha0': bool = (¬(sw_rst_i) ∧ state_changing ∧
+                                  ((fsm_state' = WaitLead) ∨ (fsm_state' = IntClockLow ∧ st.bit_counter = 0w)));
 
-	    byte_starting =  if cpha then state_changing ∧ st.byte_starting_cpha0
-                        else byte_starting_cpha0';
+	    byte_starting: bool = if cpha then state_changing ∧ st.byte_starting_cpha0
+                            else byte_starting_cpha0';
 
-
-      bit_shifting_cpha0' = ((sw_rst_i = F) ∧ state_changing ∧ (fsm_state' = IntClockLow ∧ ¬(st.bit_counter = 0w)));
+      
+      bit_shifting_cpha0': bool = (¬(sw_rst_i) ∧ state_changing ∧ (fsm_state' = IntClockLow ∧ ¬(st.bit_counter = 0w)));
 
 
 
       bit_shifting = if cpha then st.bit_shifting_cpha0 ∧ state_changing
                       else bit_shifting_cpha0';
 
-      bit_counter_d = if sw_rst_i then 0w
-                      else if ¬fsm_en then st.bit_counter
-                      else if byte_starting then start_bit
-                      else if bit_shifting then st.bit_counter - shift_size
-                      else st.bit_counter;
+      bit_counter_d: 3 word = if sw_rst_i then 0w
+                              else if ¬fsm_en then st.bit_counter
+                              else if byte_starting then start_bit
+                              else if bit_shifting then st.bit_counter - shift_size
+                              else st.bit_counter;
 
-      byte_ending_cpha0' = (¬(sw_rst_i) ∧ state_changing ∧ ((st.fsm_state = IntClockHigh) ∧ (st.bit_counter = 0w)));
-      byte_ending = if cpha then st.byte_ending_cpha0 ∧ state_changing
-                    else byte_ending_cpha0';
+      byte_ending_cpha0': bool = (¬(sw_rst_i) ∧ state_changing ∧ ((st.fsm_state = IntClockHigh) ∧ (st.bit_counter = 0w)));
+      byte_ending: bool = if cpha then st.byte_ending_cpha0 ∧ state_changing
+                          else byte_ending_cpha0';
 
-      csaat_d = if new_command then word_bit 0 command_i.csaat else st.csaat;
-      cmd_len_d = if new_command then command_i.len else st.cmd_len;
-      cmd_wr_en_d = if new_command then command_i.wr_en else st.cmd_wr_en;
+      csaat_d: bool = if new_command then word_bit 0 command_i.csaat else st.csaat;
+      cmd_len_d: 9 word = if new_command then command_i.len else st.cmd_len;
+      cmd_wr_en_d: bool = if new_command then command_i.wr_en else st.cmd_wr_en;
 
       byte_counter_d: 9 word = if sw_rst_i then 0w
                         else if ¬fsm_en then st.byte_counter
@@ -305,8 +308,8 @@ Definition spi_host_tick_def:
                         else if byte_ending then st.byte_counter - 1w
                         else st.byte_counter;
 
-      sr_wr_ready_i = st.select_valid_o;
-      wr_en_internal = (byte_starting ∧ cmd_wr_en_d);
+      sr_wr_ready_i: bool = st.select_valid_o;
+      wr_en_internal: bool = (byte_starting ∧ cmd_wr_en_d);
 
 
 
@@ -314,11 +317,11 @@ Definition spi_host_tick_def:
       merge_byte_ready_o: bool = ¬(st.merge_pos = 4); (*This is an ugly place to put this but needed for line bellow TODO: clean this up *)
 
       
-      rd_ready_o = ((¬st.rx_buf_valid) ∨ (st.rx_buf_valid ∧ merge_byte_ready_o));
-      sr_rd_ready_i = rd_ready_o;
+      rd_ready_o: bool = ((¬st.rx_buf_valid) ∨ (st.rx_buf_valid ∧ merge_byte_ready_o));
+      sr_rd_ready_i: bool = rd_ready_o;
 
       (* Back to FSM *)
-      rd_en_internal = bit_shifting;
+      rd_en_internal: bool = bit_shifting;
       tx_stall_o: bool = (wr_en_internal ∧ ¬sr_wr_ready_i);
       rx_stall_o: bool = (rd_en_internal ∧ ¬sr_rd_ready_i);
       
@@ -329,16 +332,15 @@ Definition spi_host_tick_def:
 
 
       (* byte select model*)
-      (* TODO these come from registers need to handle legit *)
       tx_data_i: 32 word = (HD st.tx_data_fifo).data;
       tx_be_i: 4 word = (HD st.tx_data_fifo).be;
       word_valid_i: bool = (LENGTH st.tx_data_fifo > 0);
       byte_ready_i: bool = wr_en_o;
 
-      byte_select_advance = (word_valid_i ∨ byte_ready_i ∨ (st.select_byte_pos > 0 ∧ word_bit (4-st.select_byte_pos) st.select_be));
+      byte_select_advance: bool = (word_valid_i ∨ byte_ready_i ∨ (st.select_byte_pos > 0 ∧ word_bit (4-st.select_byte_pos) st.select_be));
       
-      select_data' = if word_valid_i then tx_data_i else st.select_data;
-      select_be' = if word_valid_i then tx_be_i else st.select_be;
+      select_data': 32 word = if word_valid_i then tx_data_i else st.select_data;
+      select_be': 4 word = if word_valid_i then tx_be_i else st.select_be;
       
       select_byte_en: bool =  if (st.select_byte_pos > 0) then
                                 (word_bit (4-st.select_byte_pos) st.select_be)
@@ -352,7 +354,7 @@ Definition spi_host_tick_def:
                                 else st.select_byte_pos
                               else st.select_byte_pos;
 
-      select_word_ready_o = (st.select_byte_pos = 0);
+      select_word_ready_o: bool = (st.select_byte_pos = 0);
 
       select_byte_out': 8 word = if byte_select_advance then
                                   (((4-st.select_byte_pos)*8 + 7) >< ((4-st.select_byte_pos) * 8)) st.select_data
@@ -362,15 +364,15 @@ Definition spi_host_tick_def:
                               else st.select_valid_o;
       
       (* byte_merge model *)
-      (* TODO get data properlly *)
       merge_byte_in: 8 word = (7 >< 0) st.rx_buf;
       merge_valid_in: bool = st.rx_buf_valid;
       merge_word_ready_in: bool = (LENGTH st.rx_data_fifo < 64);
       
       
-      merge_byte_valid = (merge_valid_in ∨ (st.merge_pos < 4));
+      merge_byte_valid: bool = (merge_valid_in ∨ (st.merge_pos < 4));
 
-      merge_word_data': 32 word = if merge_byte_valid then (32 >< 9) (st.merge_word_data << 8) @@ merge_byte_in
+      
+      merge_word_data': 32 word = if merge_byte_valid then (((32 >< 9) (st.merge_word_data << 8)): 24 word) @@ merge_byte_in
                                   else st.merge_word_data;
       
       merge_pos': num = if merge_byte_valid then 
@@ -381,49 +383,54 @@ Definition spi_host_tick_def:
                           else st.merge_pos;
 
 
-      merge_word_o = st.merge_word_data;
+      merge_word_o: 32 word = st.merge_word_data;
       merge_word_valid_o: bool = (st.merge_pos = 4);
       merge_ready_o: bool = (st.merge_pos < 4);
       
       (*SR control *)
-      rx_ready_sr_i = merge_ready_o;
+      rx_ready_sr_i: bool = merge_ready_o;
       rx_buf_valid': bool = if sw_rst_i then F
                             else if rd_en_fsm_o ∧ rd_ready_o then T
                             else if st.rx_buf_valid ∧ rx_ready_sr_i then F
                             else st.rx_buf_valid;
 
       (* ----- End of FSM ------ *)
-      bit_counter' = if stall then st.bit_counter else bit_counter_d;
-      byte_counter' = if stall then st.byte_counter else byte_counter_d;
-      cmd_len' = if new_command ∧ ¬stall then cmd_len_d else st.cmd_len;
+      bit_counter': 3 word = if stall then st.bit_counter else bit_counter_d;
+      byte_counter': 9 word = if stall then st.byte_counter else byte_counter_d;
+      cmd_len': 9 word = if new_command ∧ ¬stall then cmd_len_d else st.cmd_len;
       
-      cmd_wr_en' = if new_command ∧ ¬stall then cmd_wr_en_d else st.cmd_wr_en;
-      csaat' = if new_command ∧ ¬stall then csaat_d else st.csaat;
+      cmd_wr_en': bool = if new_command ∧ ¬stall then cmd_wr_en_d else st.cmd_wr_en;
+      csaat': bool = if new_command ∧ ¬stall then csaat_d else st.csaat;
       
-      csid' = if new_command then command_i.csid else st.csid_q;
-      csid_q' = if new_command ∧ ¬stall then st.csid else st.csid_q;
+      csid': 1 word = if new_command then command_i.csid else st.csid_q;
+      csid_q': 1 word = if new_command ∧ ¬stall then st.csid else st.csid_q;
 
       (* Adding to data_fifos *)
-      (*TODO get from win register *)
+      (tx_word: word32, tx_be: num, q_tx: bool) = case hwext_notif of
+        SOME (Write (txdata_write be num1 word32)) => (word32, be, T)
+        | _ => (0w, 0, F);
+        
+      tx_be_w: 4 word = n2w $ tx_be;
       tx_data_new: tx_data =  <|
-        data:= 0w;
-        be:= 0w;
+        data := tx_word;
+        be := tx_be_w; 
       |>;
-      tx_ready_o = select_word_ready_o;
-      tx_data_fifo' = if tx_ready_o then APPEND st.tx_data_fifo [tx_data_new] else st.tx_data_fifo;
+      (*^For be: I don't actually know where this comes from the documentation doesn't even mention this exists *)
+      tx_ready_o: bool = (select_word_ready_o ∧ q_tx);
+      tx_data_fifo': tx_data list = if tx_ready_o then APPEND st.tx_data_fifo [tx_data_new] else st.tx_data_fifo;
 
       rx_valid: bool = merge_word_valid_o;
-      rx_data_new = merge_word_o;
-      rx_data_fifo' = if rx_valid then APPEND st.rx_data_fifo [rx_data_new] else st.rx_data_fifo;
+      rx_data_new: 32 word = merge_word_o;
+      rx_data_fifo': 32 word list = if rx_valid then APPEND st.rx_data_fifo [rx_data_new] else st.rx_data_fifo;
 
 	
       (* Errors *)
       tx_valid: bool = F; (* Need to get stuff from win reg *)
-      access_valid: bool = F; (* Need to get stuff from win reg *)
-      error_access_inval = (tx_valid ∧ ¬access_valid);
-      command_busy = (LENGTH st.commands < 64);
-      error_csid_inval = (command_valid_i ∧ command_busy ∧ ¬(st.regs.csid.csid < 1w));
-      error_cmd_inval:bool  = (command_valid_i ∧ command_busy 
+      access_valid: bool = T;
+      error_access_inval: bool = (tx_valid ∧ ¬access_valid);
+      command_busy: bool = (LENGTH st.commands < 64);
+      error_csid_inval: bool = (command_valid_i ∧ command_busy ∧ ¬(st.regs.csid.csid < 1w));
+      error_cmd_inval: bool  = (command_valid_i ∧ command_busy 
                           ∧ ¬((command_i.speed = 0w) ∨ ((command_i.speed < 3w) ∧ ¬(command_i.wr_en = command_i.rd_en))));
 
       error_overflow: bool = (tx_valid ∧ ¬tx_ready_o);
@@ -492,9 +499,9 @@ End
 Theorem spi_host_tick_buffered_notif_NONE:
   spi_host_tick notif st = INR st' ==> st'.buffered_notif = NONE
 Proof
-  simp [spi_host_tick_def]
-  >> disch_then (assume_tac o GSYM)
-  >> simp []
+  pure_rewrite_tac [spi_host_tick_def] >>
+  LET_ELIM_TAC >>
+  simp []
 QED
 
 Theorem spi_host_tick_unused_fnums:
@@ -502,8 +509,10 @@ Theorem spi_host_tick_unused_fnums:
   spi_host_tick notif (st with fnums := fnums) =
   SUM_MAP I (\st'. st' with fnums := (\i. fnums (i + n))) (spi_host_tick notif st)
 Proof
-  qexists `2`
-  >> simp [spi_host_tick_def, SF ETA_ss]
+  qexists `2` >> 
+  pure_rewrite_tac [spi_host_tick_def] >>
+  LET_ELIM_TAC >>
+  gvs [SF ETA_ss]
 QED
 
 Theorem unused_fnums_ignored_fnums_val:
